lean/Och/Soundness.lean
@@ -2,6 +2,7 @@ import Och.Syntax
 import Och.Eval
 import Och.Subtyping
 import Och.EvalSubst
+import Och.TyCheck
 import Och.Std.Unit
 import Och.Std.DBool
 
