lean/Och/Std/Unit.lean
@@ -1,6 +1,7 @@
 import Och.Macro
 import Och.Eval
 import Och.EvalSubst
+import Och.TyCheck
 
 /-!
 # Church-encoded Unit
